examples/BasePrimes.v
@@ -8,7 +8,7 @@
 
 Require Import List.
 Require Import ZArith.
-Require Import ZAux.
+Require Import ZCAux.
 
 Require Import Pock.
 
@@ -16,6 +16,10 @@ Open Local Scope positive_scope.
 
 Set Virtual Machine.
 Ltac enc t := exact_no_check t.
+
+Lemma prime2 : prime 2.
+exact prime_2.
+Qed.
 
 Lemma prime3 : prime 3.
 Proof.
