num/Lucas.v
@@ -8,20 +8,20 @@
 
 Set Implicit Arguments.
 
-Require Import ZArith.
-Require Import ZAux.
-Require Import ZDivModAux.
-Require Import Basic_type.
-Require Import ZnZ.
+Require Import ZArith Znumtheory Zpow_facts.
+Require Import CyclicAxioms DoubleCyclic BigN Cyclic31 Int31.
+Require Import ZCAux.
 Require Import W.
 Require Import Mod_op.
 Require Import LucasLehmer.
+Require Import Bits.
+Import CyclicAxioms DoubleType DoubleBase.
 
 Open Scope Z_scope. 
 
 Section test.
 
-Variable w: Set.
+Variable w: Type.
 Variable w_op: znz_op w.
 Variable op_spec: znz_spec w_op.
 Variable p: positive.
@@ -37,8 +37,8 @@ Hypothesis b_p: [|b|] = 2 ^ Zpos p - 1.
 Lemma b_pos: 0 < [|b|].
 rewrite b_p; auto with zarith.
 assert (2 ^ 0 < 2 ^ Zpos p); auto with zarith.
-apply ZAux.Zpower_lt_monotone; auto with zarith.
-rewrite ZAux.Zpower_exp_0 in H; auto with zarith.
+apply Zpower_lt_monotone; auto with zarith.
+rewrite Zpower_0_r in H; auto with zarith.
 Qed.
 
 Hint Resolve b_pos.
@@ -46,28 +46,28 @@ Hint Resolve b_pos.
 Variable m_op: mod_op w.
 Variable m_op_spec: mod_spec w_op b m_op.
 
-Let w2 := m_op.(add_mod) w_op.(znz_1) w_op.(znz_1).
+Let w2 := m_op.(add_mod) (znz_1 w_op) (znz_1 w_op).
 
-Lemma w1_b: [|w_op.(znz_1)|] = 1 mod [|b|].
-rewrite (spec_1 op_spec); simpl; auto.
-rewrite Zmod_def_small; auto with zarith.
+Lemma w1_b: [|znz_1 w_op|] = 1 mod [|b|].
+rewrite spec_1; simpl; auto.
+rewrite Zmod_small; auto with zarith.
 split; auto with zarith.
 rewrite b_p.
 assert (2 ^ 1 < 2 ^ Zpos p); auto with zarith.
-apply ZAux.Zpower_lt_monotone; auto with zarith.
-rewrite ZAux.Zpower_exp_1 in H; auto with zarith.
+apply Zpower_lt_monotone; auto with zarith.
+rewrite Zpower_1_r in H; auto with zarith.
 Qed.
 
 Lemma w2_b: [|w2|] = 2 mod [|b|].
 unfold w2; rewrite (add_mod_spec m_op_spec _ _ _ _ w1_b w1_b).
-rewrite w1_b; rewrite <- Zmod_plus; auto with zarith.
+rewrite w1_b; rewrite <- Zplus_mod; auto with zarith.
 Qed.
 
 Let w4 := m_op.(add_mod) w2 w2.
 
 Lemma w4_b: [|w4|] = 4 mod [|b|].
 unfold w4; rewrite (add_mod_spec m_op_spec _ _ _ _ w2_b w2_b).
-rewrite w2_b; rewrite <- Zmod_plus; auto with zarith.
+rewrite w2_b; rewrite <- Zplus_mod; auto with zarith.
 Qed.
 
 Let square_m2 :=
@@ -76,7 +76,7 @@ Let square_m2 :=
    fun x => sub (square x) w2.
 
 Definition lucastest :=
- w_op.(znz_to_Z) (iter_pos (Pminus p 2) _ square_m2 w4).
+ znz_to_Z w_op (iter_pos (Pminus p 2) _ square_m2 w4).
 
 Theorem lucastest_aux_correct:
  forall p1 z n, 0 <= n -> [|z|] = fst (s n) mod (2 ^ Zpos p - 1) ->
@@ -88,8 +88,8 @@ rewrite <- b_p in H.
 generalize (square_mod_spec m_op_spec _ _ H); intros H1.
 rewrite (sub_mod_spec m_op_spec _ _ _ _ H1 w2_b).
 rewrite H1; rewrite w2_b; auto with zarith.
-rewrite H; rewrite <- Zmod_mult; auto with zarith.
-rewrite <- Zmod_minus; auto with zarith.
+rewrite H; rewrite <- Zmult_mod; auto with zarith.
+rewrite <- Zminus_mod; auto with zarith.
 rewrite sn; simpl; auto with zarith.
 rewrite b_p; auto.
 intros p1 Rec w1 z Hz Hw1.
@@ -103,8 +103,8 @@ rewrite <- b_p in H1.
 generalize (square_mod_spec m_op_spec _ _ H1); intros H2.
 rewrite (sub_mod_spec m_op_spec _ _ _ _ H2 w2_b).
 rewrite H2; rewrite w2_b; auto with zarith.
-rewrite H1; rewrite <- Zmod_mult; auto with zarith.
-rewrite <- Zmod_minus; auto with zarith.
+rewrite H1; rewrite <- Zmult_mod; auto with zarith.
+rewrite <- Zminus_mod; auto with zarith.
 replace (z + Zpos (1 + p1)) with ((z + Zpos p1) + 1); auto with zarith.
 rewrite sn; simpl fst; try rewrite b_p; auto with zarith.
 rewrite Zpos_plus_distr; auto with zarith.
@@ -115,6 +115,7 @@ unfold lucastest.
 assert (F: 0 <= 0); auto with zarith.
 generalize (lucastest_aux_correct (p -2) w4 F); simpl Zplus;
    rewrite Zpos_minus; auto with zarith.
+rewrite Zmax_right; auto with zarith.
 intros tmp; apply tmp; clear tmp.
 rewrite <- b_p; simpl; exact w4_b.
 Qed.
@@ -123,8 +124,8 @@ Theorem lucastest_prop_cor: lucastest = 0 -> (2 ^ Zpos p - 1 | fst(s (Zpos p - 2
 intros H.
 apply Zmod_divide.
 assert (H1: 2 ^ 1 < 2 ^ Zpos p); auto with zarith.
-apply ZAux.Zpower_lt_monotone; auto with zarith.
-rewrite ZAux.Zpower_exp_1 in H1; auto with zarith.
+apply Zpower_lt_monotone; auto with zarith.
+rewrite Zpower_1_r in H1; auto with zarith.
 apply trans_equal with (2:= H); apply sym_equal; apply lucastest_prop; auto.
 Qed.
 
@@ -132,80 +133,39 @@ Theorem lucastest_prime:  lucastest = 0 -> prime (2 ^ Zpos p - 1).
 intros H1; case (prime_dec (2 ^ Zpos p - 1)); auto; intros H2.
 case Zdivide_div_prime_le_square with (2 := H2).
 assert (H3: 2 ^ 1 < 2 ^ Zpos p); auto with zarith.
-apply ZAux.Zpower_lt_monotone; auto with zarith.
-rewrite ZAux.Zpower_exp_1 in H3; auto with zarith.
+apply Zpower_lt_monotone; auto with zarith.
+rewrite Zpower_1_r in H3; auto with zarith.
 intros q (H3, (H4, H5)).
 contradict H5; apply Zlt_not_le.
 generalize q_more_than_square; unfold Mp; intros tmp; apply tmp;
   auto; clear tmp.
 apply lucastest_prop_cor; auto.
 case (Zle_lt_or_eq 2 q); auto.
-apply prime_le_2; auto.
+apply prime_ge_2; auto.
 intros H5; subst.
 absurd (2 <= 1); auto with arith.
 apply Zdivide_le; auto with zarith.
 case H4; intros x Hx.
 exists (2 ^ (Zpos p -1) - x).
 rewrite Zmult_minus_distr_r; rewrite <- Hx; unfold Mp.
-pattern 2 at 2; rewrite <- Zpower_exp_1; rewrite <- Zpower_exp; auto with zarith.
+pattern 2 at 2; rewrite <- Zpower_1_r; rewrite <- Zpower_exp; auto with zarith.
 replace (Zpos p - 1 + 1) with (Zpos p); auto with zarith.
 Qed.
 
 End test.
 
-Definition znz_of_Z (w:Set) (op:znz_op w) z :=
+Definition znz_of_Z (w: Type) (op: znz_op w) z :=
  match z with
- | Zpos p => snd (op.(znz_of_pos) p)
- | _ => op.(znz_0)
+ | Zpos p => snd (znz_of_pos op p)
+ | _ => znz_0 op
  end.
 
-Fixpoint plength (p: positive) : positive :=
-  match p with 
-    xH => xH
-  | xO p1 => Psucc (plength p1)
-  | xI p1 => Psucc (plength p1)
-  end.
-
 Definition lucas p :=
- let op := cmk_op (nat_of_P (plength p) - 3) in
+ let op := cmk_op (pred (nat_of_P (get_height 31 p))) in
  let b := znz_of_Z op (Zpower 2 (Zpos p) - 1) in
- let mod_op := mmake_mod_op op b p (2 * op.(znz_digits) - p) in
+ let zp := znz_of_Z op (Zpos p) in
+ let mod_op := mmake_mod_op op b zp in
   lucastest op p mod_op.
-
-Time Eval compute in lucas 127.
-
-Theorem plength_correct: forall p, (Zpos p < 2 ^ Zpos (plength p))%Z.
-assert (F: (forall p, 2 ^ (Zpos (Psucc p)) = 2 * 2 ^ Zpos p)%Z).
-intros p; replace (Zpos (Psucc p)) with (1 + Zpos p)%Z.
-rewrite Zpower_exp; auto with zarith.
-rewrite Zpos_succ_morphism; unfold Zsucc; auto with zarith.
-intros p; elim p; simpl plength; auto.
-intros p1 Hp1; rewrite F; repeat rewrite Zpos_xI.
-assert (tmp: (forall p, 2 * p = p + p)%Z); 
-  try repeat rewrite tmp; auto with zarith.
-intros p1 Hp1; rewrite F; rewrite (Zpos_xO p1).
-assert (tmp: (forall p, 2 * p = p + p)%Z); 
-  try repeat rewrite tmp; auto with zarith.
-rewrite ZPowerAux.Zpower_exp_1; auto with zarith.
-Qed.
-
-Theorem plength_pred_correct: forall p, (Zpos p <= 2 ^ Zpos (plength (Ppred p)))%Z.
-intros p; case (Psucc_pred p); intros H1.
-subst; simpl plength.
-rewrite ZPowerAux.Zpower_exp_1; auto with zarith.
-pattern p at 1; rewrite <- H1.
-rewrite Zpos_succ_morphism; unfold Zsucc; auto with zarith.
-generalize (plength_correct (Ppred p)); auto with zarith.
-Qed.
-
-Definition pheight p := plength (Ppred (plength (Ppred p))).
-
-Theorem pheight_correct: forall p, (Zpos p <= 2 ^ (2 ^ (Zpos (pheight p))))%Z.
-intros p; apply Zle_trans with (1 := (plength_pred_correct p)).
-apply ZPowerAux.Zpower_le_monotone; auto with zarith.
-split; auto with zarith.
-unfold pheight; apply plength_pred_correct.
-Qed.
 
 Theorem lucas_prime:
  forall p, 2 < Zpos p -> lucas p = 0 -> prime (2 ^ Zpos p - 1).
@@ -214,45 +174,40 @@ match type of H with lucastest (cmk_op ?x) ?y ?z = _ =>
    set (w_op := (cmk_op x)); assert(A1: znz_spec w_op)
 end.
 unfold w_op; apply cmk_spec.
-assert (F0: p <= znz_digits w_op).
-unfold w_op, base; rewrite (cmk_op_digits (nat_of_P (plength p) - 3)).
-apply Zle_trans with (2 ^ plength p).
-apply Zlt_le_weak; apply plength_correct.
-apply Zpower_le_monotone; auto with zarith.
-split; auto with zarith.
-case (le_or_lt 3 (nat_of_P (plength p))); intros A2.
-rewrite inj_minus1; simpl; auto with zarith.
+assert (F0: Zpos p <= Zpos (znz_digits w_op)).
+unfold w_op, base; rewrite (cmk_op_digits (pred (nat_of_P (get_height 31 p)))).
+generalize (get_height_correct 31 p).
+replace (Z_of_nat (pred (nat_of_P (get_height 31 p)))) with
+       ((Zpos (get_height 31 p) - 1) ); auto with zarith.
+rewrite pred_of_minus; rewrite inj_minus1; auto with zarith.
 rewrite <- Zpos_eq_Z_of_nat_o_nat_of_P; auto with zarith.
-rewrite inj_minus2; simpl; auto with zarith.
-generalize (inj_le (nat_of_P (plength p)) 3); simpl; auto with zarith.
-rewrite <- Zpos_eq_Z_of_nat_o_nat_of_P; auto with zarith.
-assert (F1: znz_to_Z w_op (znz_of_Z w_op (2 ^ p - 1)) = 2 ^ p - 1).
-assert (F1: 0 < 2 ^ p - 1).
-assert (F2: 2 ^ 0 < 2 ^ p); auto with zarith.
+generalize (lt_O_nat_of_P (get_height 31 p)); auto with zarith.
+assert (F1: znz_to_Z w_op (znz_of_Z w_op (2 ^ (Zpos p) - 1)) = 2 ^ (Zpos p) - 1).
+assert (F1: 0 < 2 ^ (Zpos p) - 1).
+assert (F2: 2 ^ 0 < 2 ^ (Zpos p)); auto with zarith.
 apply Zpower_lt_monotone; auto with zarith.
-rewrite Zpower_exp_0 in F2; auto with zarith.
-case_eq (2 ^ p - 1); simpl znz_to_Z.
+rewrite Zpower_0_r in F2; auto with zarith.
+case_eq (2 ^ (Zpos p) - 1); simpl znz_to_Z.
 intros HH; contradict F1; rewrite HH; auto with zarith.
 2: intros p1 HH; contradict F1; rewrite HH; 
   apply Zle_not_lt; red; simpl; intros; discriminate.
 intros p1 Hp1; apply znz_of_pos_correct; auto.
 rewrite <- Hp1.
 unfold base.
-apply Zlt_le_trans with (2 ^ p); auto with zarith.
+apply Zlt_le_trans with (2 ^ (Zpos p)); auto with zarith.
 apply Zpower_le_monotone; auto with zarith.
 match type of H with lucastest (cmk_op ?x) ?y ?z = _ =>
-   apply (fun U V =>
-    @lucastest_prime _ _ (cmk_spec x) p (znz_of_Z (cmk_op x) 
-                 (2 ^ Zpos p  -1)) U V z)
+  apply  
+  (@lucastest_prime _ _ (cmk_spec x) p (znz_of_Z w_op (2 ^ Zpos p  -1)) Hp F1 z)
 end; auto with zarith; fold w_op.
-apply mmake_mod_spec; auto with zarith.
-rewrite F1.
-assert (F2: 2 ^ 1 < 2 ^p); auto with zarith.
+eapply mmake_mod_spec with (p := p); auto with zarith.
+unfold znz_of_Z; unfold znz_of_Z in F1; rewrite F1.
+assert (F2: 2 ^ 1 < 2 ^ (Zpos p)); auto with zarith.
 apply Zpower_lt_monotone; auto with zarith.
-rewrite Zpower_exp_1 in F2; auto with zarith.
-rewrite Zpos_minus; auto with zarith.
-rewrite Zmisc.Zpos_mult; auto with zarith.
-rewrite (Zpos_xO (znz_digits w_op)); auto with zarith.
-rewrite Zmisc.Zpos_mult; auto with zarith.
+rewrite Zpower_1_r in F2; auto with zarith.
+rewrite znz_of_Z_correct; auto with zarith.
+split; auto with zarith.
+apply Zle_lt_trans with (1 := F0); auto with zarith.
+unfold base; apply Zpower2_lt_lin; auto with zarith.
 Qed.
 
